New semantics for regions, along with SCF semantics.
This mega-commit introduces new semantics for regions,
and uses these to provide semantics for arith, scf, cf. These
semantics are designed to show that the only thing an op can
do with a region is to execute it.

MLIR/Semantics/Fitree.lean
@@ -106,18 +106,17 @@ def Fitree.bind {E R T} (t: Fitree E T) (k: T → Fitree E R) :=
   | Ret r => k r
   | Vis e k' => Vis e (fun r => bind (k' r) k)
 
-#check Functor
 def Fitree.map {E } (f: α → β) (fa: Fitree E α): Fitree E β :=
    match fa with
    | .Ret r => .Ret (f r)
    | .Vis e k' => .Vis e (fun r => map f (k' r))
 
-theorem Fitree_map_functorial (f: α → β) (g: β → γ) (fa: Fitree E α): 
+theorem Fitree_map_functorial (f: α → β) (g: β → γ) (fa: Fitree E α):
    fa.map (g ∘ f) = (fa.map f).map g := by {
   intros;
   unfold Fitree.map;
   induction fa;
-  simp; 
+  simp;
   unfold Fitree.map;
   simp;
   case Vis IH => {
@@ -128,7 +127,7 @@ theorem Fitree_map_functorial (f: α → β) (g: β → γ) (fa: Fitree E α):
    apply IH;
   }
 }
-  
+
 instance {E}: Monad (Fitree E) where
   pure := Fitree.ret
   bind := Fitree.bind
@@ -151,7 +150,7 @@ theorem Fitree_monad_right_identity (ma: Fitree E α):
   simp;
   funext x; -- classical
   unfold Fitree.bind;
-  case Vis IH => 
+  case Vis IH =>
   apply IH;
 }
 
@@ -180,35 +179,38 @@ def Fitree.translate {E F R} (f: E ~> F): Fitree E R → Fitree F R
 -- Interpretation into the monad of finite ITrees
 @[simp_itree]
 def interp {M} [Monad M] {E} (h: E ~> M):
-    forall ⦃R⦄, Fitree E R → M R :=
-  fun _ t =>
+    forall {R}, Fitree E R → M R :=
+  fun t =>
     match t with
     | Fitree.Ret r => pure r
     | Fitree.Vis e k => bind (h _ e) (fun t => interp h (k t))
 
 @[simp_itree]
 def interp' {E F} (h: E ~> Fitree PVoid):
-    forall ⦃R⦄, Fitree (E +' F) R → Fitree F R :=
-  fun _ t =>
+    forall {R}, Fitree (E +' F) R → Fitree F R :=
+  fun t =>
     interp (Fitree.case_
       (fun _ e => (h _ e).translate $ fun _ e => nomatch e)
       (fun _ e => Fitree.trigger e)) t
 
--- Interpretation into the state monad
--- NOTE: This is semantically equivalent to interp,
--- but it is easier to state theorems about `interp_state`, instead of
--- stating theorems about `@interp (StateT S)`.
+-- Interpretation into the state monad. This is semantically equivalent to
+-- `interp`, but the specialization is useful to write state-specific theorems.
 @[simp_itree]
 def interp_state {M S} [Monad M] {E} (h: E ~> StateT S M):
-    forall ⦃R⦄, Fitree E R → StateT S M R :=
+    forall {R}, Fitree E R → StateT S M R :=
   interp h
 
 -- Interpretation into the writer monad
 @[simp_itree]
-def interp_writer [Monad M] {E} (h: E ~> WriterT M):
-    forall ⦃R⦄, Fitree E R → WriterT M R :=
+def interp_writer {M} [Monad M] {E} (h: E ~> WriterT M):
+    forall {R}, Fitree E R → WriterT M R :=
   interp h
 
+-- Interpretation into the option monad
+@[simp_itree]
+def interp_option {M} [Monad M] {E} (h: E ~> OptionT M):
+    forall {R}, Fitree E R → OptionT M R :=
+  interp h
 
 -- Since we only use finite ITrees, we can actually run them when they're
 -- fully interpreted (which leaves only the Ret constructor)
@@ -240,4 +242,7 @@ elab "simp_itree" : tactic => do
   let lemmas := (← SimpItreeExtension.getTheorems).toUnfold.fold
     (init := #[]) (fun acc n => acc.push (toSimpLemma n))
   evalTactic $ ← `(tactic|simp [$lemmas.reverse,*,
-    Member.inject, StateT.bind, StateT.pure, bind, pure, cast_eq])
+    Member.inject,
+    StateT.bind, StateT.pure, StateT.lift,
+    OptionT.bind, OptionT.pure, OptionT.mk, OptionT.lift,
+    bind, pure, cast_eq, Eq.mpr])
