MLIR/Semantics/Semantics.lean
@@ -13,94 +13,190 @@ import MLIR.AST
 open MLIR.AST
 
 
-inductive BlockResult {Gα Gσ Gε} (Gδ: Dialect Gα Gσ Gε)
+inductive BlockResult {α σ ε} (δ: Dialect α σ ε)
 | Branch (bb: BBName) (args: List SSAVal)
-| Ret (rets: List (SSAVal × MLIRType Gδ))
-| Next
+| Ret (rets:  List ((τ : MLIRType δ) × MLIRType.eval τ))
+| Next (val: (τ: MLIRType δ) × τ.eval)
 
-instance (Gδ: Dialect Gα Gσ Gε): ToString (BlockResult Gδ) where
+instance : Inhabited (BlockResult δ) where
+  default := .Ret []
+
+instance (δ: Dialect α σ ε): ToString (BlockResult δ) where
   toString := fun
     | .Branch bb args => s!"Branch {bb} {args}"
-    | .Ret rets => s!"Ret {rets}"
-    | .Next => "Next"
+    | .Ret rets       => s!"Ret {rets}"
+    | .Next ⟨τ, val⟩  => s!"Next {val}: {τ}"
 
-class Semantics {α σ ε} (δ: Dialect α σ ε) where
-  -- Events modeling the dialect's operations
+-- Interpreted operation, like MLIR.AST.Op, but with less syntax
+inductive IOp (δ: Dialect α σ ε) := | mk
+  (name:    String)
+  (args:    List ((τ: MLIRType δ) × τ.eval))
+  (bbargs:  List BBName)
+  (regions: Nat)
+  (attrs:   AttrDict δ)
+  (type:    MLIRType δ)
+
+-- Effect to run a region
+-- TODO: change this to also deal with scf.if and yield.
+inductive RegionE (Δ: Dialect α' σ' ε'): Type -> Type
+| RunRegion (ix: Nat): RegionE Δ (BlockResult Δ)
+
+class Semantics (δ: Dialect α σ ε)  where
+  -- Events modeling the dialect's computational behavior. Usually operations
+  -- are simply denoted by a trigger of such an event. This excludes, however,
+  -- operations that have regions or otherwise call into other dialects, since
+  -- every operation in the program must be accessible before we start
+  -- interpreting.
   E: Type → Type
 
-  -- Operation semantics function: maps an `Op` to an interaction tree. Usually
-  -- this simply emits an event of `E` and records the return value into the
-  -- environment, and could be automated.
-  semantics_op {Gα Gσ Gε} {Gδ: Dialect Gα Gσ Gε}:
-    Option SSAVal → Op Gδ → Option (Fitree (SSAEnvE Gδ +' E) (BlockResult Gδ))
+  -- Operation semantics function: maps an IOp (morally an Op but slightly less
+  -- rich to guarantee good properties) to an interaction tree. Usually exposes
+  -- any region calls then emits of event of E. This function runs on the
+  -- program's entire dialect Δ but returns none for any operation that is not
+  -- part of δ.
+  semantics_op:
+    IOp Δ →
+    Option (Fitree (RegionE Δ +' UBE +' E) (BlockResult Δ))
 
   -- TODO: Allow a dialects' semantics to specify their terminators along with
   -- TODO| their branching behavior, instead of hardcoding it for cf
 
   -- Event handler used when interpreting the operations and running programs.
-  -- This is where most of the semantics and computations take place.
+  -- This is where most of the computational semantics take place.
   -- TODO: Allow dialect handlers to emit events into other dialects
   handle: E ~> Fitree PVoid
 
-instance {α₁ σ₁ ε₁} {δ₁: Dialect α₁ σ₁ ε₁} {α₂ σ₂ ε₂} {δ₂: Dialect α₂ σ₂ ε₂}
-    [S₁: Semantics δ₁] [S₂: Semantics δ₂]: Semantics (δ₁ + δ₂) where
+
+-- The memory of a smaller dialect can be injected into a larger one.
+
+mutual
+variable (Δ: Dialect α' σ' ε') [S: Semantics Δ]
+
+def denoteOp (op: Op Δ):
+    Fitree (UBE +' SSAEnvE Δ +' S.E) (BlockResult Δ) :=
+  match op with
+  | .mk name args0 bbargs regions0 attrs (.fn (.tuple τs) t) => do
+      -- Read arguments from memory
+      let args ← (List.zip args0 τs).mapM (fun (name, τ) => do
+          return ⟨τ, ← Fitree.trigger <| SSAEnvE.Get τ name⟩)
+      -- Evaluate regions
+      let regions := denoteRegions regions0
+      -- Built the interpreted operation
+      let iop : IOp Δ := IOp.mk name args bbargs regions0.length attrs (.fn (.tuple τs) t)
+      -- Use the dialect-provided semantics, and substitute regions
+      match S.semantics_op iop with
+      | some t =>
+          interp (fun _ e =>
+            match e with
+            | Sum.inl (RegionE.RunRegion ix) => regions.get! ix
+            | Sum.inr <| Sum.inl ube => Fitree.trigger ube
+            | Sum.inr <| Sum.inr se => Fitree.trigger se
+          ) t
+      | none => do
+          Fitree.trigger <| UBE.DebugUB s!"invalid op: {op}"
+          return default
+
+  | _ => do
+      Fitree.trigger <| UBE.DebugUB s!"invalid denoteOp: {op}"
+      return .Next ⟨.unit, ()⟩
+
+def denoteBBStmt (bbstmt: BasicBlockStmt Δ):
+    Fitree (UBE +' SSAEnvE Δ +' S.E) (BlockResult Δ) :=
+  match bbstmt with
+  | .StmtAssign val _ op => do
+      let br ← denoteOp op
+      match br with
+      | .Next ⟨τ, v⟩ =>
+          Fitree.trigger (SSAEnvE.Set τ val v)
+      | _ =>
+          Fitree.trigger (UBE.DebugUB s!"invalid denoteBBStmt: {bbstmt}")
+      return br
+  | .StmtOp op =>
+      denoteOp op
+
+def denoteBB (bb: BasicBlock Δ):
+    Fitree (UBE +' SSAEnvE Δ +' S.E) (BlockResult Δ) :=
+  -- TODO: Bind basic block arguments before running the basic block
+  -- TODO: Any checks on the BlockResults of intermediate ops?
+  match bb with
+  | .mk name args [] =>
+      return BlockResult.Next ⟨.unit, ()⟩
+  | .mk name args [stmt] =>
+      denoteBBStmt stmt
+  | .mk name args (stmt :: stmts) => do
+      let _ ← denoteBBStmt stmt
+      denoteBB (.mk name args stmts)
+
+def denoteRegion (r: Region Δ):
+    Fitree (UBE +' SSAEnvE Δ +' S.E) (BlockResult Δ) :=
+  -- We only define semantics for single-basic-block regions
+  -- TODO: Pass region arguments
+  -- TODO: Forward region's return type and value
+  match r with
+  | .mk [bb] =>
+      denoteBB bb
+  | _ => do
+      Fitree.trigger (UBE.DebugUB s!"invalid denoteRegion (>1 bb): {r}")
+      return BlockResult.Next ⟨.unit, ()⟩
+
+def denoteRegions (l: List (Region Δ)):
+    List (Fitree (UBE +' SSAEnvE Δ +' S.E) (BlockResult Δ)) :=
+  match l with
+  | [] => []
+  | r::l => denoteRegion r :: denoteRegions l
+end
+
+
+instance
+    {α₁ σ₁ ε₁} {δ₁: Dialect α₁ σ₁ ε₁}
+    {α₂ σ₂ ε₂} {δ₂: Dialect α₂ σ₂ ε₂}
+    [S₁: Semantics δ₁]
+    [S₂: Semantics δ₂]
+    : Semantics (δ₁ + δ₂) where
   E := S₁.E +' S₂.E
-  semantics_op ret_name op :=
-    (S₁.semantics_op ret_name op).map (.translate Member.inject) <|>
-    (S₂.semantics_op ret_name op).map (.translate Member.inject)
+  semantics_op op :=
+    (S₁.semantics_op op).map (.translate Member.inject) <|>
+    (S₂.semantics_op op).map (.translate Member.inject)
   handle := Fitree.case_ S₁.handle S₂.handle
 
-def semantics_op! {Gα Gσ Gε} {Gδ: Dialect Gα Gσ Gε} [S: Semantics Gδ]:
-    Option SSAVal → Op Gδ →
-    Fitree (UBE +' SSAEnvE Gδ +' S.E) (BlockResult Gδ) :=
-  fun ret op =>
-    match S.semantics_op ret op with
-    | some t => t.translate Member.inject
-    | none => do Fitree.trigger (UBE.DebugUB s!"{op}"); return .Next
-
-def semantics_bbstmt {Gα Gσ Gε} {Gδ: Dialect Gα Gσ Gε} [S: Semantics Gδ]:
-    BasicBlockStmt Gδ →
-    Fitree (UBE +' SSAEnvE Gδ +' S.E) (BlockResult Gδ)
-| .StmtAssign val _ op => semantics_op! (some val) op
-| .StmtOp op => semantics_op! none op
-
--- TODO: Add the basic block arguments and bind them before running the block
-def semantics_bb {Gα Gσ Gε} {Gδ: Dialect Gα Gσ Gε} [S: Semantics Gδ]
-    (bb: BasicBlock Gδ):
-    Fitree (UBE +' SSAEnvE Gδ +' S.E) (BlockResult Gδ) := do
-  -- TODO: we assume all statements return BlockResult.Next except the last
-  for stmt in bb.stmts.init do
-    let _ ← semantics_bbstmt stmt
-  match bb.stmts.getLast? with
-  | some stmt => semantics_bbstmt stmt
-  | none => return BlockResult.Next
-
-def semantics_region_go {Gα Gσ Gε} {Gδ: Dialect Gα Gσ Gε} [S: Semantics Gδ]
-    (fuel: Nat) (r: Region Gδ) (bb: BasicBlock Gδ):
-    Fitree (UBE +' SSAEnvE Gδ +' S.E) (BlockResult Gδ) :=
+def semanticsRegionRec
+    [inst: CoeDialect δ Δ]
+    [S: Semantics Δ]
+    (fuel: Nat) (r: Region δ) (bb: BasicBlock δ):
+    Fitree (UBE +' SSAEnvE Δ +' S.E) (BlockResult Δ) :=
   match fuel with
-  | 0 => return .Next
+  | 0 => return .Next ⟨.unit, ()⟩
   | fuel' + 1 => do
-      match ← semantics_bb bb with
+      match ← denoteBB Δ bb with
         | .Branch bbname args =>
             -- TODO: Pass the block arguments
             match r.getBasicBlock bbname with
-            | some bb' => semantics_region_go fuel' r bb'
-            | none => return .Next
+            | some bb' => semanticsRegionRec fuel' r bb'
+            | none => return .Next ⟨.unit, ()⟩
         | .Ret rets => return .Ret rets
-        | .Next => return .Next
+        | .Next v => return .Next v
 
 -- TODO: Pass region arguments
 -- TODO: Forward region's return type and value
-def semantics_region {Gα Gσ Gε} {Gδ: Dialect Gα Gσ Gε} [S: Semantics Gδ]
+def semanticsRegion {Gα Gσ Gε} {Gδ: Dialect Gα Gσ Gε} [S: Semantics Gδ]
     (fuel: Nat) (r: Region Gδ):
     Fitree (UBE +' SSAEnvE Gδ +' S.E) Unit := do
-  let _ ← semantics_region_go fuel r (r.bbs.get! 0)
+  let _ ← semanticsRegionRec fuel r (r.bbs.get! 0)
 
-def run {Gα Gσ Gε} {Gδ: Dialect Gα Gσ Gε} [S: Semantics Gδ] {R}
-    (t: Fitree (UBE +' SSAEnvE Gδ +' S.E) R) (env: SSAEnv Gδ):
-    R × SSAEnv Gδ :=
+
+
+def run! {Δ: Dialect α' σ' ε'} [S: Semantics Δ] {R}
+    (t: Fitree (UBE +' SSAEnvE Δ +' S.E) R) (env: SSAEnv Δ):
+    R × SSAEnv Δ :=
   let t := interp_ub! t
+  let t := interp_ssa t env
+  let t := interp S.handle t
+  t.run
+
+def run {Δ: Dialect α' σ' ε'} [S: Semantics Δ] {R}
+    (t: Fitree (UBE +' SSAEnvE Δ +' S.E) R) (env: SSAEnv Δ):
+    Option R × SSAEnv Δ :=
+  let t := interp_ub t
   let t := interp_ssa t env
   let t := interp S.handle t
   t.run
@@ -113,11 +209,11 @@ def runLogged {Gα Gσ Gε} {Gδ: Dialect Gα Gσ Gε} [S: Semantics Gδ]
   let t := interp S.handle t
   t.run
 
+
 /-
 ### Denotation notation
 -/
 
-#print Op
 class Denote (δ: Dialect α σ ε) [S: Semantics δ]
     (T: {α σ: Type} → {ε: σ → Type} → Dialect α σ ε → Type) where
   denote: T δ → Fitree (UBE +' SSAEnvE δ +' S.E) (BlockResult δ)
@@ -125,12 +221,13 @@ class Denote (δ: Dialect α σ ε) [S: Semantics δ]
 notation "⟦ " t " ⟧" => Denote.denote t
 
 instance (δ: Dialect α σ ε) [Semantics δ]: Denote δ Op where
-  denote op := semantics_op! none op
+  denote op := denoteOp δ op
 
 instance (δ: Dialect α σ ε) [Semantics δ]: Denote δ BasicBlockStmt where
-  denote := semantics_bbstmt
+  denote bbstmt := denoteBBStmt δ bbstmt
 
 instance (δ: Dialect α σ ε) [Semantics δ]: Denote δ BasicBlock where
-  denote := semantics_bb
+  denote bb := denoteBB δ bb
+
 
 -- Not for regions because we need to specify the fuel
