MLIR/Dialects/ScfSemantics.lean
@@ -1,0 +1,63 @@
+import MLIR.Semantics.Fitree
+import MLIR.Semantics.Semantics
+import MLIR.Semantics.SSAEnv
+import MLIR.Semantics.UB
+import MLIR.Util.Metagen
+import MLIR.AST
+import MLIR.EDSL
+open MLIR.AST
+
+/-
+### Dialect: `scf`
+-/
+
+instance scf: Dialect Void Void (fun x => Unit) where
+  iα := inferInstance
+  iε := inferInstance
+
+-- Operations of `scf` that unfold into regions need to expose these regions
+-- immediately at denotation time rather than at interpretation time, so that
+-- inner operations can be interpreted correctly. So operations with regions
+-- are not represented here, and handled directly in `semantics_op`.
+inductive ScfE: Type -> Type :=
+
+-- | run a loop, decrementing i from n to -
+-- | ix := lo + (n - i) * step
+def run_loop_bounded_go [Monad m] (n: Nat) (i: Nat) (lo: Int) (step: Int)
+  (accum: a) (eff: Int -> a -> m a): m a := do
+   let ix : Int := lo + (n - i) * step
+   let accum <- eff ix accum
+   match i with
+   | .zero => return accum
+   | .succ i' => run_loop_bounded_go n i' lo step accum eff
+
+-- | TODO: use this to run regions.
+def run_loop_bounded [Monad m] (n: Nat) (lo: Int) (step: Int) (accum: a) (eff: Int -> a -> m a): m a :=
+  run_loop_bounded_go n n lo step accum eff
+
+-- | TODO: refactor to (1) an effect, (2) an interpretation
+-- | TODO: use the return type of Scf.For. For now, just do unit.
+def scf_semantics_op: IOp Δ →
+      Option (Fitree (RegionE Δ +' UBE +' ScfE) (BlockResult Δ))
+  | IOp.mk "scf.for" [⟨.i32, lo⟩, ⟨.i32, hi⟩, ⟨.i32, step⟩] [] 1 _ _ => some do
+    let nsteps : Int := ((FinInt.toSint'  hi) - (FinInt.toSint' lo)) / FinInt.toSint' step
+    run_loop_bounded
+      (a := BlockResult Δ)
+      (n := nsteps.toNat)
+      (lo := (FinInt.toSint' lo))
+      (step := (FinInt.toSint' step))
+      (accum := default)
+      (eff := (fun i _ => Fitree.trigger <| RegionE.RunRegion 0))
+  | _ => none
+
+def handleScf: ScfE ~> Fitree PVoid :=
+  fun _ e => nomatch e
+
+instance: Semantics scf where
+  E := ScfE
+  semantics_op := scf_semantics_op
+  handle := handleScf
+
+/-
+### Examples and testing
+-/
